remove time methods from grove FFI

src/goose_lang/lib/time/impl.v
@@ -11,6 +11,7 @@ Module time.
     Definition Millisecond: val := #1000000.
     Definition Second: val := #1000000000.
     Definition Sleep: val := λ: "duration", #().
+    Definition TimeNow: val := λ: <>, #0. (* FIXME make it actually nondet *)
     Definition AfterFunc: val := λ: "duration" "f", Fork "f" ;; ref "f".
     Definition Timer__Reset: val := λ: "timer", !"timer" #(). (* FIXME: this could rerun f *)
   End goose_lang.
